src/arch/x64/X64.Leakage_Ins_Xmm_i.fst
@@ -5,29 +5,30 @@ open X64.Taint_Semantics_s
 open X64.Leakage_s
 open X64.Leakage_Helpers_i
 open Types_s
+open Words_s
 open TypesNative_s
 open FStar.FunctionalExtensionality
 
 let xmm_taint (ts:taintState) (x:xmm) = ts.xmmTaint x
 
 let set_xmm_taint (ts:taintState) (xmm:xmm) (taint:taint) : taintState =
-  TaintState ts.regTaint ts.flagsTaint (fun x -> if x = xmm then taint else ts.xmmTaint x)
+  TaintState ts.regTaint ts.flagsTaint ts.cfFlagsTaint (fun x -> if x = xmm then taint else ts.xmmTaint x)
 
 #set-options "--z3rlimit 20"
   
-val quad32_xor_lemma: (x:quad32) -> Lemma (quad32_xor x x == Quad32 0 0 0 0) 
+val quad32_xor_lemma: (x:quad32) -> Lemma (quad32_xor x x == Mkfour 0 0 0 0) 
 
 let quad32_xor_lemma x =
-  assert (quad32_xor x x == Quad32 (nat32_xor x.lo x.lo) (nat32_xor x.mid_lo x.mid_lo)
-    (nat32_xor x.mid_hi x.mid_hi) (nat32_xor x.hi x.hi));
-  TypesNative_s.reveal_ixor 32 x.lo x.lo;
-  TypesNative_s.reveal_ixor 32 x.mid_lo x.mid_lo;
-  TypesNative_s.reveal_ixor 32 x.mid_hi x.mid_hi;
-  TypesNative_s.reveal_ixor 32 x.hi x.hi;
-  FStar.UInt.logxor_self #32 x.lo;
-  FStar.UInt.logxor_self #32 x.mid_lo;
-  FStar.UInt.logxor_self #32 x.mid_hi;
-  FStar.UInt.logxor_self #32 x.hi
+  assert (quad32_xor x x == Mkfour (nat32_xor x.lo0 x.lo0) (nat32_xor x.lo1 x.lo1)
+    (nat32_xor x.hi2 x.hi2) (nat32_xor x.hi3 x.hi3));
+  TypesNative_s.reveal_ixor 32 x.lo0 x.lo0;
+  TypesNative_s.reveal_ixor 32 x.lo1 x.lo1;
+  TypesNative_s.reveal_ixor 32 x.hi2 x.hi2;
+  TypesNative_s.reveal_ixor 32 x.hi3 x.hi3;
+  FStar.UInt.logxor_self #32 x.lo0;
+  FStar.UInt.logxor_self #32 x.lo1;
+  FStar.UInt.logxor_self #32 x.hi2;
+  FStar.UInt.logxor_self #32 x.hi3
 
 val check_if_pxor_leakage_free: (ins:tainted_ins{let i, _, _ = ins.ops in Pxor? i}) -> (ts:taintState) -> (res:(bool*taintState){let b, ts' = res in b2t b ==>
      isConstantTime (Ins ins) ts /\ isLeakageFree (Ins ins) ts ts'})
@@ -37,12 +38,12 @@ let check_if_pxor_leakage_free ins ts =
   if src = dst then begin
     let ts' = set_xmm_taint ts dst Public in
     Classical.forall_intro quad32_xor_lemma;
-    true, TaintState ts'.regTaint Secret ts'.xmmTaint
+    true, TaintState ts'.regTaint Secret Secret ts'.xmmTaint
   end 
   else begin
     let taint = merge_taint (xmm_taint ts dst) (xmm_taint ts src) in
     let ts' = set_xmm_taint ts dst taint in
-    true, TaintState ts'.regTaint Secret ts'.xmmTaint
+    true, TaintState ts'.regTaint Secret Secret ts'.xmmTaint
   end
 
 val check_if_paddd_leakage_free: (ins:tainted_ins{let i, _, _ = ins.ops in Paddd? i}) -> (ts:taintState) -> (res:(bool*taintState){let b, ts' = res in b2t b ==>
@@ -52,7 +53,7 @@ let check_if_paddd_leakage_free ins ts =
   let Paddd dst src, _, _ = ins.ops in
   let taint = merge_taint (xmm_taint ts dst) (xmm_taint ts src) in
   let ts' = set_xmm_taint ts dst taint in
-  true, TaintState ts'.regTaint Secret ts'.xmmTaint
+  true, TaintState ts'.regTaint Secret Secret ts'.xmmTaint
 
 val check_if_pslld_leakage_free: (ins:tainted_ins{let i, _, _ = ins.ops in Pslld? i}) -> (ts:taintState) -> (res:(bool*taintState){let b, ts' = res in b2t b ==>
      isConstantTime (Ins ins) ts /\ isLeakageFree (Ins ins) ts ts'})
@@ -61,7 +62,7 @@ let check_if_pslld_leakage_free ins ts =
   let Pslld dst amt, _, _ = ins.ops in
   let taint = xmm_taint ts dst in
   let ts' = set_xmm_taint ts dst taint in
-  true, TaintState ts'.regTaint Secret ts'.xmmTaint
+  true, TaintState ts'.regTaint Secret Secret ts'.xmmTaint
 
 val check_if_psrld_leakage_free: (ins:tainted_ins{let i, _, _ = ins.ops in Psrld? i}) -> (ts:taintState) -> (res:(bool*taintState){let b, ts' = res in b2t b ==>
      isConstantTime (Ins ins) ts /\ isLeakageFree (Ins ins) ts ts'})
@@ -70,7 +71,7 @@ let check_if_psrld_leakage_free ins ts =
   let Psrld dst amt, _, _ = ins.ops in
   let taint = xmm_taint ts dst in
   let ts' = set_xmm_taint ts dst taint in
-  true, TaintState ts'.regTaint Secret ts'.xmmTaint
+  true, TaintState ts'.regTaint Secret Secret ts'.xmmTaint
 
 val check_if_pshufb_leakage_free: (ins:tainted_ins{let i, _, _ = ins.ops in Pshufb? i}) -> (ts:taintState) -> (res:(bool*taintState){let b, ts' = res in b2t b ==>
      isConstantTime (Ins ins) ts /\ isLeakageFree (Ins ins) ts ts'})
@@ -79,7 +80,7 @@ let check_if_pshufb_leakage_free ins ts =
   let Pshufb dst src, _, _ = ins.ops in
   let taint = merge_taint (xmm_taint ts dst) (xmm_taint ts src) in
   let ts' = set_xmm_taint ts dst taint in
-  true, TaintState ts'.regTaint Secret ts'.xmmTaint
+  true, TaintState ts'.regTaint Secret Secret ts'.xmmTaint
 
 val check_if_pshufd_leakage_free: (ins:tainted_ins{let i, _, _ = ins.ops in Pshufd? i}) -> (ts:taintState) -> (res:(bool*taintState){let b, ts' = res in b2t b ==>
      isConstantTime (Ins ins) ts /\ isLeakageFree (Ins ins) ts ts'})
@@ -88,19 +89,20 @@ let check_if_pshufd_leakage_free ins ts =
   let Pshufd dst src _, _, _ = ins.ops in
   let taint = merge_taint (xmm_taint ts dst) (xmm_taint ts src) in
   let ts' = set_xmm_taint ts dst taint in
-  true, TaintState ts'.regTaint Secret ts'.xmmTaint
+  true, TaintState ts'.regTaint Secret Secret ts'.xmmTaint
 
 val check_if_pinsrd_leakage_free: (ins:tainted_ins{let i, _, _ = ins.ops in Pinsrd? i}) -> (ts:taintState) -> (res:(bool*taintState){let b, ts' = res in b2t b ==>
      isConstantTime (Ins ins) ts /\ isLeakageFree (Ins ins) ts ts'})
 
 let check_if_pinsrd_leakage_free ins ts =
-  let Pinsrd dst src _, _, _ = ins.ops in
-  let fixedTime = operand_does_not_use_secrets src ts in
-  assert (fixedTime ==> isConstantTime (Ins ins) ts);
-  let taint = merge_taint (xmm_taint ts dst) (operand_taint src ts) in
-  let taint = merge_taint taint ins.t in
-  let ts' = set_xmm_taint ts dst taint in
-  fixedTime, TaintState ts'.regTaint Secret ts'.xmmTaint
+  false, ts
+  // let Pinsrd dst src _, _, _ = ins.ops in
+  // let fixedTime = operand_does_not_use_secrets src ts in
+  // assert (fixedTime ==> isConstantTime (Ins ins) ts);
+  // let taint = merge_taint (xmm_taint ts dst) (operand_taint src ts) in
+  // let taint = merge_taint taint ins.t in
+  // let ts' = set_xmm_taint ts dst taint in
+  // fixedTime, TaintState ts'.regTaint Secret Secret ts'.xmmTaint
 
 val check_if_vpslldq_leakage_free: (ins:tainted_ins{let i, _, _ = ins.ops in VPSLLDQ? i}) -> (ts:taintState) -> (res:(bool*taintState){let b, ts' = res in b2t b ==>
      isConstantTime (Ins ins) ts /\ isLeakageFree (Ins ins) ts ts'})
@@ -109,7 +111,7 @@ let check_if_vpslldq_leakage_free ins ts =
   let VPSLLDQ dst src _, _, _ = ins.ops in
   let taint = merge_taint (xmm_taint ts dst) (xmm_taint ts src) in
   let ts' = set_xmm_taint ts dst taint in
-  true, TaintState ts'.regTaint Secret ts'.xmmTaint
+  true, TaintState ts'.regTaint Secret Secret ts'.xmmTaint
 
 val check_if_pclmuldqd_leakage_free: (ins:tainted_ins{let i, _, _ = ins.ops in Pclmulqdq? i}) -> (ts:taintState) -> (res:(bool*taintState){let b, ts' = res in b2t b ==>
      isConstantTime (Ins ins) ts /\ isLeakageFree (Ins ins) ts ts'})
@@ -120,7 +122,7 @@ let check_if_pclmuldqd_leakage_free ins ts =
   let Pclmulqdq dst src _, _, _ = ins.ops in
   let taint = merge_taint (xmm_taint ts dst) (xmm_taint ts src) in
   let ts' = set_xmm_taint ts dst taint in
-  true, TaintState ts'.regTaint Secret ts'.xmmTaint
+  true, TaintState ts'.regTaint Secret Secret ts'.xmmTaint
 
 val check_if_aesni_enc_leakage_free: (ins:tainted_ins{let i, _, _ = ins.ops in AESNI_enc? i}) -> (ts:taintState) -> (res:(bool*taintState){let b, ts' = res in b2t b ==>
      isConstantTime (Ins ins) ts /\ isLeakageFree (Ins ins) ts ts'})
@@ -129,7 +131,7 @@ let check_if_aesni_enc_leakage_free ins ts =
   let AESNI_enc dst src, _, _ = ins.ops in
   let taint = merge_taint (xmm_taint ts dst) (xmm_taint ts src) in
   let ts' = set_xmm_taint ts dst taint in
-  true, TaintState ts'.regTaint Secret ts'.xmmTaint
+  true, TaintState ts'.regTaint Secret Secret ts'.xmmTaint
 
 val check_if_aesni_enc_last_leakage_free: (ins:tainted_ins{let i, _, _ = ins.ops in AESNI_enc_last? i}) -> (ts:taintState) -> (res:(bool*taintState){let b, ts' = res in b2t b ==>
      isConstantTime (Ins ins) ts /\ isLeakageFree (Ins ins) ts ts'})
@@ -138,7 +140,7 @@ let check_if_aesni_enc_last_leakage_free ins ts =
   let AESNI_enc_last dst src, _, _ = ins.ops in
   let taint = merge_taint (xmm_taint ts dst) (xmm_taint ts src) in
   let ts' = set_xmm_taint ts dst taint in
-  true, TaintState ts'.regTaint Secret ts'.xmmTaint
+  true, TaintState ts'.regTaint Secret Secret ts'.xmmTaint
 
 val check_if_aesni_dec_leakage_free: (ins:tainted_ins{let i, _, _ = ins.ops in AESNI_dec? i}) -> (ts:taintState) -> (res:(bool*taintState){let b, ts' = res in b2t b ==>
      isConstantTime (Ins ins) ts /\ isLeakageFree (Ins ins) ts ts'})
@@ -147,7 +149,7 @@ let check_if_aesni_dec_leakage_free ins ts =
   let AESNI_dec dst src, _, _ = ins.ops in
   let taint = merge_taint (xmm_taint ts dst) (xmm_taint ts src) in
   let ts' = set_xmm_taint ts dst taint in
-  true, TaintState ts'.regTaint Secret ts'.xmmTaint
+  true, TaintState ts'.regTaint Secret Secret ts'.xmmTaint
 
 val check_if_aesni_dec_last_leakage_free: (ins:tainted_ins{let i, _, _ = ins.ops in AESNI_dec_last? i}) -> (ts:taintState) -> (res:(bool*taintState){let b, ts' = res in b2t b ==>
      isConstantTime (Ins ins) ts /\ isLeakageFree (Ins ins) ts ts'})
@@ -156,7 +158,7 @@ let check_if_aesni_dec_last_leakage_free ins ts =
   let AESNI_dec_last dst src, _, _ = ins.ops in
   let taint = merge_taint (xmm_taint ts dst) (xmm_taint ts src) in
   let ts' = set_xmm_taint ts dst taint in
-  true, TaintState ts'.regTaint Secret ts'.xmmTaint
+  true, TaintState ts'.regTaint Secret Secret ts'.xmmTaint
 
 val check_if_aesni_imc_leakage_free: (ins:tainted_ins{let i, _, _ = ins.ops in AESNI_imc? i}) -> (ts:taintState) -> (res:(bool*taintState){let b, ts' = res in b2t b ==>
      isConstantTime (Ins ins) ts /\ isLeakageFree (Ins ins) ts ts'})
@@ -165,7 +167,7 @@ let check_if_aesni_imc_leakage_free ins ts =
   let AESNI_imc dst src, _, _ = ins.ops in
   let taint = merge_taint (xmm_taint ts dst) (xmm_taint ts src) in
   let ts' = set_xmm_taint ts dst taint in
-  true, TaintState ts'.regTaint Secret ts'.xmmTaint
+  true, TaintState ts'.regTaint Secret Secret ts'.xmmTaint
 
 val check_if_aesni_keygen_leakage_free: (ins:tainted_ins{let i, _, _ = ins.ops in AESNI_keygen_assist? i}) -> (ts:taintState) -> (res:(bool*taintState){let b, ts' = res in b2t b ==>
      isConstantTime (Ins ins) ts /\ isLeakageFree (Ins ins) ts ts'})
@@ -174,7 +176,7 @@ let check_if_aesni_keygen_leakage_free ins ts =
   let AESNI_keygen_assist dst src _, _, _ = ins.ops in
   let taint = merge_taint (xmm_taint ts dst) (xmm_taint ts src) in
   let ts' = set_xmm_taint ts dst taint in
-  true, TaintState ts'.regTaint Secret ts'.xmmTaint
+  true, TaintState ts'.regTaint Secret Secret ts'.xmmTaint
 
 val check_if_xmm_ins_consumes_fixed_time: (ins:tainted_ins{is_xmm_ins ins}) -> (ts:taintState) -> (res:(bool*taintState){ins_consumes_fixed_time ins ts res})
 
@@ -197,4 +199,5 @@ let check_if_xmm_ins_consumes_fixed_time ins ts =
     | AESNI_dec_last dst src -> check_if_aesni_dec_last_leakage_free ins ts
     | AESNI_imc dst src -> check_if_aesni_imc_leakage_free ins ts
     | AESNI_keygen_assist dst src imm -> check_if_aesni_keygen_leakage_free ins ts
+    | _ -> false, ts // Unsupported yet
     
